systems/chord-props/LiveNodePreservation.v
@@ -65,10 +65,37 @@ Proof.
 Qed.
 Hint Resolve live_node_preserved_by_tick.
 
+Lemma live_node_join_exists_after_simple_change :
+  forall h src dst l succs gst gst' st st',
+    live_node_in_msg_succ_lists gst ->
+    In (src, (dst, GotSuccList succs)) l ->
+    (forall x, In x l -> In x (msgs gst)) ->
+    nodes gst = nodes gst' ->
+    failed_nodes gst = failed_nodes gst' ->
+    sigma gst h = Some st ->
+    sigma gst' = update addr_eq_dec (sigma gst) h (Some st') ->
+    joined st = joined st' ->
+    length succs > 0 ->
+    Exists (live_node gst') (map addr_of succs).
+Proof.
+  intros.
+  assert (Exists (live_node gst) (map addr_of succs)).
+  {
+    unfold live_node_in_msg_succ_lists in *; break_and.
+    find_eapply_prop live_node_in_msg_succ_lists_join; eauto.
+  }
+  apply Exists_exists; find_apply_lem_hyp Exists_exists.
+  break_exists_exists; split; break_and; auto.
+  break_live_node.
+  destruct (addr_eq_dec x h); subst;
+    eapply live_node_characterization;
+    repeat find_rewrite; rewrite_update; try find_injection; eauto.
+Qed.
+
 Lemma live_node_exists_after_simple_change :
   forall h src dst l succs gst gst' st st',
     live_node_in_msg_succ_lists gst ->
-    (exists p, In (src, (dst, GotPredAndSuccs p succs)) l) \/ In (src, (dst, GotSuccList succs)) l ->
+    (exists p, In (src, (dst, GotPredAndSuccs p succs)) l) ->
     (forall x, In x l -> In x (msgs gst)) ->
     nodes gst = nodes gst' ->
     failed_nodes gst = failed_nodes gst' ->
@@ -78,18 +105,19 @@ Lemma live_node_exists_after_simple_change :
     length succs > 0 ->
     Exists (live_node gst') (map addr_of (chop_succs (make_pointer src :: succs))).
 Proof.
-  repeat (match goal with H: _ |- _ => clear H end).
   intros.
-  assert (Exists (live_node gst) (map addr_of (chop_succs (make_pointer src :: succs))))
-    by (repeat break_or_hyp; break_exists;
-        eapply_prop live_node_in_msg_succ_lists; eauto).
+  break_exists.
+  assert (Exists (live_node gst) (map addr_of (chop_succs (make_pointer src :: succs)))).
+  {
+    unfold live_node_in_msg_succ_lists in *; break_and.
+    find_eapply_prop live_node_in_msg_succ_lists'; eauto.
+  }
   apply Exists_exists; find_apply_lem_hyp Exists_exists.
   break_exists_exists; split; break_and; auto.
   break_live_node.
-  destruct (addr_eq_dec x h); subst;
+  destruct (addr_eq_dec x0 h); subst;
     eapply live_node_characterization;
     repeat find_rewrite; rewrite_update; try find_injection; eauto.
-  Unshelve. exact None.
 Qed.
 
 Lemma live_node_not_just_started :
